deps/coq-poulet4/lib/P4cub/TypeSoundness.v
@@ -1,3 +1,4 @@
+Require Import Coq.micromega.Lia.
 Require Import P4cub.Value.
 Require Import P4cub.BigStep.
 Module P := P4cub.AST.P4cub.
@@ -10,24 +11,92 @@ Import Step.
 Import P.P4cubNotations.
 Import V.ValueNotations.
 Import V.ValueTyping.
+Import F.FieldTactics.
 
-Section Theorems.
+Section BigStepTheorems.
   Context {tags_t : Type}.
 
   (** Epsilon's values type's agree with Gamma. *)
   Definition envs_type (errs : errors) (Γ : gamma) (ϵ : epsilon) : Prop :=
     forall (x : name tags_t) (τ : E.t tags_t) (v : V.v tags_t),
-      Γ x = Some τ -> ϵ x = Some v /\ ∇ errs ⊢ v ∈ τ.
+      Γ x = Some τ -> ϵ x = Some v -> ∇ errs ⊢ v ∈ τ.
   (**[]*)
 
-  (* TODO: figure out how to use notations...*)
   Theorem big_step_preservation :
-    forall (errs : errors) (Γ : gamma) (e : E.e tags_t) (τ : E.t tags_t)
-      (ϵ : epsilon) (v : V.v tags_t),
+    forall (errs : errors) (Γ : gamma) (e : E.e tags_t)
+      (τ : E.t tags_t) (ϵ : epsilon) (v : V.v tags_t),
       envs_type errs Γ ϵ ->
       ⟨ ϵ, e ⟩ ⇓ v ->
       ⟦ errs, Γ ⟧ ⊢ e ∈ τ ->
       ∇ errs ⊢ v ∈ τ.
   Proof.
+    intros errs Γ e τ ϵ v Het Hev.
+    generalize dependent τ.
+    unfold envs_type in Het.
+    induction Hev using custom_expr_big_step_ind;
+      intros t Ht; inv Ht; try constructor; eauto.
+    - inv H2; auto.
+    - unfold BitArith.neg;  unfold BitArith.bound;
+        unfold BitArith.maxN; unfold BitArith.upper_bound. admit.
+    - unfold IntArith.bound; unfold IntArith.neg;
+      unfold IntArith.return_bound; unfold IntArith.maxZ;
+        unfold IntArith.minZ. admit.
+    - apply IHHev1 in H10; auto; clear IHHev1.
+      apply IHHev2 in H11; auto; clear IHHev2.
+      destruct op; unfold eval_bit_binop in *;
+        inv H; inv H9; constructor; admit.
+    - destruct op; unfold eval_bool_binop in *;
+        inv H; inv H9; constructor.
+    - unfold eval_bit_binop in *; inv H; constructor.
+    - unfold eval_bit_binop in *; inv H; constructor.
+    - unfold eval_bit_binop in *; inv H; constructor.
+    - inv H10.
+    - inv H10.
+    - inv H8; constructor. admit.
+    - apply IHHev1 in H10; auto; clear IHHev1.
+      apply IHHev2 in H11; auto; clear IHHev2.
+      destruct op; unfold eval_bit_binop in *;
+        inv H; inv H9; constructor; admit.
+    - destruct op; unfold eval_bool_binop in *;
+        inv H; inv H9; constructor.
+    - inv H; constructor.
+    - inv H; constructor.
+    - inv H9.
+    - inv H9.
+    - pose proof IHHev Het _ H6 as IH; clear IHHev.
+      inv IH. Search (In _ ?l -> Forall2 _ ?l _ -> _).
+      (** TODO: Need lemma:
+          [forall R x1 l1 l2, In x1 l1 -> Forall2 R l1 l2 -> exists x2, In x2 l2 /\ R x1 x2],
+          and some Field-specific lemma:
+          [forall x a1 a2 l1 l2 R, F.get x l1 = Some a1 -> F.get x l2 = a2 ->]
+          [F.relfs R l1 l2 -> R a1 a2] *) admit.
+    - admit.
+    - generalize dependent tfs; rename H0 into Hesvs.
+      induction H; inv Hesvs;
+        intros ts Hests; inv Hests; constructor.
+      destruct x as [x [τ e]]; destruct y as [y v];
+        destruct y0 as [z t]; repeat invert_relf; simpl in *.
+      + split; simpl;
+          try (transitivity x; auto; symmetry; assumption);
+          destruct H2; auto.
+      + apply IHForall2; auto.
+    - clear e H6 IHHev Hev.
+      generalize dependent tfs; rename H0 into Hesvs.
+      induction H; inv Hesvs;
+        intros ts Hests; inv Hests; constructor.
+      destruct x as [x [τ e]]; destruct y as [y v];
+        destruct y0 as [z t]; repeat invert_relf; simpl in *.
+      + split; simpl;
+          try (transitivity x; auto; symmetry; assumption);
+          destruct H2; auto.
+      + apply IHForall2; auto.
+    - destruct op; simpl in *; constructor;
+        pose proof IHHev Het _ H5 as IH; clear IHHev; inv IH; auto.
+    - admit.
+    - clear n ni H5 H7 H8.
+      rename H0 into Hhsvss; rename H9 into Hhs.
+      induction H; inv Hhsvss; inv Hhs; constructor;
+        destruct y as [b vs]; eauto.
+    - (* TODO: about a specific header in the header stack. *) admit.
   Abort.
-End Theorems.
+End BigStepTheorems.
